src/coq/optimisations/paco_util.v
@@ -1,30 +1,313 @@
-Require Import paco.
-Require Import Vellvm.Effects.
-Require Import Vellvm.StepSemantics.
-Require Import Vellvm.Ollvm_ast.
-Require Import Vellvm.Memory.
-Require Import Vellvm.Effects.
 Require Import ZArith List String Omega.
 Require Import  Vellvm.Ollvm_ast Vellvm.Classes Vellvm.Util Vellvm.CFGProp Vellvm.CFG.
+Require Import Vellvm.optimisations.wellformedSSA.
+Require Import Vellvm.optimisations.transform.
+Require Import Vellvm.optimisations.add_instr.
+Require Import paco.
+Require Import Vellvm.Memory.
+Require Import Vellvm.Effects.
+From mathcomp.ssreflect
+Require Import ssreflect ssrbool seq eqtype ssrnat.
 
 
-Set Implicit Arguments.
-Set Contextual Implicit.
 
-Module A : Vellvm.StepSemantics.ADDR with Definition addr := nat.
-  Definition addr := nat.
-End A.  
+Print mcfg.
 
-Module SS := StepSemantics.StepSemantics(A).
-Export SS.
 
-Ltac finish X :=
-repeat match goal with
-  | [ |- trace_equiv_step (upaco2 (trace_equiv_step (X:=())) _) (Vis (trace_map (fun _ : state => ()) <$> Err _)) (Vis (trace_map (fun _ : state => ()) <$> Err _)) ] => constructor; constructor
-  | [ |- related_event_step (upaco2 (trace_equiv_step (X:=())) _) (Vis (trace_map (fun _ : state => ()) <$> Err _)) (Vis (trace_map (fun _ : state => ()) <$> Err _)) ] => constructor
-  | [ |- trace_equiv_step (upaco2 (trace_equiv_step (X:=())) _) (Vis (trace_map (fun _ : state => ()) <$> Fin _)) (Vis (trace_map (fun _ : state => ()) <$> Fin _)) ] => constructor; constructor; auto
-  | [ |- trace_equiv_step (upaco2 (trace_equiv_step (X:=())) _) (Tau () (memD _ (trace_map (fun _ : state => ()) (step_sem _ _)))) (Tau () (memD _ (trace_map (fun _ : state => ()) (step_sem _ _))))] => constructor; right; apply X
 
+
+
+Print cfg.
+Print block.
+Print block_id.
+Print raw_id.
+
+Print int.
+
+
+Lemma test : forall n, n + 1 = n + 2.
+Proof. Admitted.
+
+
+
+
+Hint Resolve test.
+
+
+Lemma test1 : forall n, n + 1 = n + 2.
+Proof. auto. Admitted.
+
+
+Definition unroll (t:Trace ()) :=
+match t with
+  | Vis a => Vis a
+  | Tau a b => Tau a b
 end.
 
-Ltac destr_simpl P X:= destruct P; simpl; finish X.
+
+
+
+Lemma trace_equiv_err : forall s0 s1 r, trace_equiv_step (upaco2 (trace_equiv_step (X:=())) r)
+  (Vis (trace_map (fun _ : state => ()) <$> Err s0))
+  (Vis (trace_map (fun _ : state => ()) <$> Err s1)).
+Proof. intros. constructor. constructor. Qed.
+
+Hint Resolve trace_equiv_err.
+
+
+
+Lemma trace_equiv_fin : forall s0 r, trace_equiv_step (upaco2 (trace_equiv_step (X:=())) r)
+  (Vis (trace_map (fun _ : state => ()) <$> Fin s0))
+  (Vis (trace_map (fun _ : state => ()) <$> Fin s0)).
+Proof. intros. constructor. constructor. auto. Qed.
+
+Hint Resolve trace_equiv_fin.
+
+
+Lemma trace_equiv_tau_left : forall (d1 d2:Trace ()), trace_equiv d1 d2 -> trace_equiv (Tau () d1) d2.
+Proof. intros. pfold. constructor. punfold H. Qed.
+
+Hint Resolve trace_equiv_tau_left.
+
+Lemma trace_equiv_tau_right : forall (d1 d2:Trace ()), trace_equiv d1 d2 -> trace_equiv d1 (Tau () d2).
+Proof. intros. pfold. constructor. punfold H. Qed.
+
+Hint Resolve trace_equiv_tau_right.
+
+
+
+Lemma trace_equiv_tau : forall (r:Trace () -> Trace () -> Prop) (A B: Trace ()) (CIH: r (A) (B)) ,
+trace_equiv_step (upaco2 (trace_equiv_step (X:=())) r)   (Tau ()
+     (A))
+  (Tau ()
+     (B)).
+Proof. intros.
+constructor. right. apply CIH. Qed. 
+
+
+
+Hint Resolve trace_equiv_tau.
+
+
+Lemma trace_refl1 : forall (a:Trace ())
+, trace_equiv a a.
+Proof. pcofix CIH. intros. pfold. destruct a. destruct v. simpl. constructor. constructor. auto.
+constructor. constructor. constructor. constructor.
+destruct e. simpl.
+  +constructor. right. subst. apply CIH.
+  +constructor. auto. right. subst. eauto.
+  +constructor. auto. auto. right. eauto.
+  +constructor. auto. auto. right. subst. apply CIH.
+constructor. right. apply CIH. Qed.
+
+
+Hint Resolve trace_refl1.
+
+
+
+Lemma trace_refl2 : forall (r:Trace () -> Trace () -> Prop) (CIH: forall (b c: Trace()), r b c) (a:Trace ()),
+trace_equiv_step (upaco2 (trace_equiv_step (X:=())) r) a a.
+Proof.
+ intros.
+ destruct a. destruct v.
+  +constructor. constructor. auto.
+  +constructor. constructor.
+  +constructor. destruct e.
+    -constructor. constructor. right; subst. apply CIH.
+    -constructor. constructor. auto. right; subst. apply CIH.
+    -constructor. constructor. auto. auto. right. apply CIH.
+    -constructor. constructor. auto. auto. right. subst. apply CIH.
+  +constructor. right. apply CIH.
+Qed.
+
+
+
+
+
+
+Hint Resolve trace_refl2.
+
+Print Step.
+Print state.
+
+
+Definition generic_start D prog mem e s fn bk iid :=
+  match
+    match
+      match
+        match D with
+        | Step s' =>
+            Tau ({| fn := fn; bk := bk; pt := iid |}, e, s)
+              (step_sem prog s')
+        | Jump s' =>
+            Tau ({| fn := fn; bk := bk; pt := iid |}, e, s)
+              (step_sem prog s')
+        | Obs (Fin s0) => Vis (Fin s0)
+        | Obs (Err s0) => Vis (Err s0)
+        | Obs (Eff m) => Vis (Eff (effects_map (step_sem prog) m))
+        end
+      with
+      | Vis v => Vis (trace_map (fun _ : state => ()) <$> v)
+      | Tau _ k => Tau () (trace_map (fun _ : state => ()) k)
+      end
+    with
+    | Vis (Fin _ as x) => Vis x
+    | Vis (Err _ as x) => Vis x
+    | Vis (Eff e0) =>
+        match mem_step e0 mem with
+        | inl e1 => Vis (Eff e1)
+        | inr (m', v, k) => Tau () (memD m' (k v))
+        end
+    | Tau x d' => Tau x (memD mem d')
+    end
+  with
+  | Vis a => Vis a
+  | Tau a b => Tau a b
+  end
+.
+
+
+Definition generic_step prog mem C p e s fn bk (id:local_id) :=
+generic_start (do dv <- C; Step (p, add_env id dv e, s)) prog mem e s fn bk (IId id)
+.
+
+Definition generic_function_entry_error f s0 prog mem e s fn bk id :=
+generic_start (let 'FunctionEntry _ _ := f in Obs (Err s0)) prog mem e s fn bk id.
+(*          (do st <- jump prog (fn p) (bk p) br e s;
+           Jump st)*)
+Print pc.
+
+
+
+
+
+Lemma generic_step_refl : forall  (r: Trace () -> Trace () -> Prop) (CIH: forall (st : state) (prog : mcfg)
+        (mem : memory),
+      r (memD mem (sem prog st))
+        (memD mem (sem prog st)))
+C prog mem s id e p fn bk, trace_equiv_step (upaco2 (trace_equiv_step (X:=())) r) 
+(generic_step prog mem C p e s fn bk id) (generic_step prog mem C p e s fn bk id).
+Proof. intros. unfold generic_step, generic_start.
+destruct C; simpl; eauto. Qed.
+
+
+Hint Resolve generic_step_refl.
+
+
+
+
+Lemma generic_function_entry_refl : forall  (r: Trace () -> Trace () -> Prop) (CIH: forall (st : state) (prog : mcfg)
+        (mem : memory),
+      r (memD mem (sem prog st))
+        (memD mem (sem prog st)))
+prog mem s0 f s id e fn bk, trace_equiv_step (upaco2 (trace_equiv_step (X:=())) r) 
+(generic_function_entry_error f s0 prog mem e s fn bk id) (generic_function_entry_error f s0 prog mem e s fn bk id).
+Proof. intros. unfold generic_function_entry_error, generic_start.
+destruct f; simpl; eauto. Qed.
+
+
+Hint Resolve generic_function_entry_refl.
+Print pc.
+
+(*
+        match
+          match f with
+          | KRet _ _ _ =>
+              t_raise_p p
+                "IMPOSSIBLE: Ret void in non-return configuration"
+          | KRet_void e' p' => Jump (p', e', s)
+          end
+        with
+        | Step s' => Tau (p, e, f :: s) (step_sem prog s')
+        | Jump s' => Tau (p, e, f :: s) (step_sem prog s')
+        | Obs (Fin s0) => Vis (Fin s0)
+        | Obs (Err s0) => Vis (Err s0)
+        | Obs (Eff m) => Vis (Eff (effects_map (step_sem prog) m))
+        end*)
+
+Definition jump_solve prog mem e s p br2:=
+  match
+    match
+      match
+        match (do st <- jump prog (fn p) (bk p) br2 e s; Jump st) with
+        | Step s' => Tau (p, e, s) (step_sem prog s')
+        | Jump s' => Tau (p, e, s) (step_sem prog s')
+        | Obs (Fin s0) => Vis (Fin s0)
+        | Obs (Err s0) => Vis (Err s0)
+        | Obs (Eff m) => Vis (Eff (effects_map (step_sem prog) m))
+        end
+      with
+      | Vis v0 => Vis (trace_map (fun _ : state => ()) <$> v0)
+      | Tau _ k => Tau () (trace_map (fun _ : state => ()) k)
+      end
+    with
+    | Vis (Fin _ as x0) => Vis x0
+    | Vis (Err _ as x0) => Vis x0
+    | Vis (Eff e0) =>
+        match mem_step e0 mem with
+        | inl e1 => Vis (Eff e1)
+        | inr (m', v0, k) => Tau () (memD m' (k v0))
+        end
+    | Tau x0 d' => Tau x0 (memD mem d')
+    end
+  with
+  | Vis a => Vis a
+  | Tau a b => Tau a b
+  end
+.
+
+
+
+Lemma generic_jump_refl : forall  (r: Trace () -> Trace () -> Prop) (CIH: forall (st : state) (prog : mcfg)
+        (mem : memory),
+      r (memD mem (sem prog st))
+        (memD mem (sem prog st)))
+prog mem s e p br2, trace_equiv_step (upaco2 (trace_equiv_step (X:=())) r) 
+(jump_solve prog mem e s p br2) (jump_solve prog mem e s p br2).
+Proof. intros. unfold jump_solve. destruct (jump prog (fn p) (bk p) br2 e s); simpl; eauto. Qed. 
+
+Hint Resolve generic_jump_refl.
+
+Lemma trace_refl123 : forall st prog mem, trace_equiv (memD mem (sem (prog) st)) (memD mem (sem (prog) st)).
+Proof. pcofix CIH. intros. pfold.
+assert ((memD mem (sem prog st)) = unroll (memD mem (sem prog st))). destruct (memD mem (sem prog st)); eauto.
+rewrite H. simpl.
+unfold stepD. simpl. destruct st; simpl; eauto. destruct p; simpl; eauto.
+destruct (fetch prog p); simpl; eauto. destruct c; simpl; eauto. destruct (incr_pc prog p); simpl; eauto.
+destruct p; simpl; eauto. destruct pt; simpl; eauto. destruct i; simpl; eauto.
+destruct (eval_op e None op); simpl; eauto.
+destruct (fn0); simpl; eauto. destruct i; simpl; eauto.
+
+destruct ((find_function_entry prog id0)); simpl; eauto.
+destruct (           map_monad (fun '(t0, op) => eval_op e (Some t0) op)); simpl; eauto.
+eapply generic_function_entry_refl; eauto.
+destruct ((find_function_entry prog id0)); simpl; eauto.
+destruct f; simpl; eauto.
+destruct f; simpl; eauto.
+destruct ptr; simpl; eauto.
+destruct (eval_op e (Some t0) v); simpl; eauto.
+destruct v0; simpl; eauto.
+destruct i; simpl; eauto. destruct fn0; simpl; eauto.
+destruct i; simpl; eauto. 
+destruct ((find_function_entry prog id)); simpl; eauto.
+destruct f; simpl; eauto.
+destruct (map_monad (fun '(t0, op) => eval_op e (Some t0) op) args); simpl; eauto.
+destruct t; simpl; eauto.
+destruct val, ptr; simpl; eauto.
+
+destruct (eval_op e (Some t) v); simpl; eauto.
+destruct (eval_op e (Some t0) v0); simpl; eauto.
+destruct v2; simpl; eauto.
+destruct t; simpl; eauto.
+destruct v; simpl; eauto.
+destruct (eval_op e (Some t) v); simpl; eauto.
+destruct s; simpl; eauto.
+destruct f; simpl; eauto.
+destruct s; simpl; eauto.
+destruct f; simpl; eauto.
+destruct v; simpl; eauto.
+destruct (eval_op e (Some t) v); simpl; eauto.
+destruct v0; simpl; eauto.
+ destruct (StepSemantics.Int1.eq x StepSemantics.Int1.one); simpl; eauto;
+eapply generic_jump_refl; eauto.
+Admitted.
