src/coq/optimisations/congruence2.v
@@ -1,0 +1,666 @@
+Require Import ZArith List String Omega.
+Require Import  Vellvm.Ollvm_ast Vellvm.Classes Vellvm.Util Vellvm.CFGProp Vellvm.CFG.
+Require Import Vellvm.optimisations.wellformedSSA.
+Require Import Vellvm.optimisations.transform.
+Require Import Vellvm.optimisations.add_instr.
+Require Import Vellvm.optimisations.paco_util.
+Require Import Vellvm.optimisations.step_trace.
+Require Import Vellvm.DecidableEquality.
+Require Import Coq.Logic.FunctionalExtensionality.
+Require Import paco.
+Require Import Vellvm.Memory.
+Require Import Vellvm.Effects.
+From mathcomp.ssreflect
+Require Import ssreflect ssrbool seq eqtype ssrnat.
+
+
+
+Print mcfg.
+
+
+Definition unroll (t:Trace ()) :=
+match t with
+  | Vis a => Vis a
+  | Tau a b => Tau a b
+end.
+
+
+
+Print cfg.
+Print block.
+
+(*If all the functions are equal, then the execution is the same*)
+
+
+Print find_function.
+
+Definition function_equal :=
+forall m1 m2 fid, find_function m1 fid = find_function m2 fid.
+
+
+
+Definition jump_equal_trace_equiv := forall m1 m2 fn bk br2 e s, jump m1 fn bk br2 e s = jump m2 fn bk br2 e s.
+
+
+Lemma jump_equal : function_equal -> jump_equal_trace_equiv.
+Proof. unfold function_equal, jump_equal_trace_equiv.
+intros.
+unfold jump. simpl. unfold find_block_entry.
+simpl.
+generalize (H m1 m2 fn). intros. rewrite H0. simpl. destruct (find_function m2 fn); eauto. Qed.
+
+
+
+
+
+Lemma function_equal_trace_equiv : (function_equal) -> forall mem m1 m2 s, (trace_equiv (memD mem (sem m1 s)) (memD mem (sem m2 s))).
+Proof. intro func_equal. pcofix CIH. intros. pfold.
+
+
+assert (memD mem (sem m1 s) = unroll (memD mem (sem m1 s))).
+destruct (memD mem (sem m1 s)); simpl; eauto.
+rewrite H. clear H.
+
+
+assert ((memD mem (sem m2 s)) = unroll (memD mem (sem m2 s))). destruct (memD mem (sem m2 s)); eauto. rewrite H; clear H.
+unfold function_equal in func_equal. destruct s. destruct p. destruct p.
+simpl. unfold find_function_entry. simpl.
+
+
+
+generalize (func_equal m1 m2 fn). intros. 
+remember (find_function m1 fn) as A.
+remember (find_function m2 fn) as B.
+destruct A, B; simpl; inversion H; simpl; eauto. subst.
+destruct ( find_block (blks (df_instrs d0)) bk); simpl; eauto.
+destruct (block_to_cmd b pt); simpl; eauto.
+destruct p; simpl; eauto.
+destruct c; simpl; eauto.
+destruct o; simpl; eauto.
+destruct pt; simpl; eauto.
+destruct i; simpl; eauto.
+destruct (eval_op e None op); simpl; eauto.
+destruct fn0; simpl; eauto.
+destruct i; simpl; eauto.
+generalize (func_equal m1 m2 id0); intros; simpl; eauto. inversion H0.
+destruct (find_function m1 id0); simpl; eauto.
+simpl. destruct (find_block (blks (df_instrs d)) (init (df_instrs d))); simpl; eauto.
+destruct ( map_monad (fun '(t0, op) => eval_op e (Some t0) op) args); simpl; eauto.
+destruct ptr; simpl; eauto. destruct (eval_op e (Some t0) v); simpl; eauto.
+destruct v0; simpl; eauto.
+destruct i; simpl; eauto.
+destruct fn0; simpl; eauto.
+destruct i; simpl; eauto.
+generalize (func_equal m1 m2 id); intros; simpl; eauto. inversion H0.
+destruct (find_function m1 id ); simpl; eauto.
+destruct (find_block (blks (df_instrs d)) (init (df_instrs d))); simpl; eauto.
+destruct (map_monad (fun '(t0, op) => eval_op e (Some t0) op) args); simpl; eauto.
+destruct t; simpl; eauto.
+destruct val; simpl; eauto.
+destruct ptr; simpl; eauto.
+destruct (eval_op e (Some t) v); simpl; eauto.
+destruct (eval_op e (Some t0) v0); simpl; eauto.
+destruct v2; simpl; eauto.
+destruct t; simpl; eauto.
+destruct v; simpl; eauto.
+destruct (eval_op e (Some t) v); simpl; eauto.
+destruct s; simpl; eauto.
+destruct f; simpl; eauto.
+destruct s; simpl; eauto.
+destruct f; simpl; eauto.
+destruct v; simpl; eauto.
+destruct (eval_op e (Some t) v); simpl; eauto.
+destruct v0; simpl; eauto.
+destruct (StepSemantics.Int1.eq x StepSemantics.Int1.one); simpl; eauto.
+apply jump_equal in func_equal. unfold jump_equal_trace_equiv in func_equal.
+specialize (func_equal m1 m2 fn bk br1 e s). rewrite func_equal.
+destruct (jump m2 fn bk br1 e s); simpl; eauto.
+apply jump_equal in func_equal. unfold jump_equal_trace_equiv in func_equal.
+specialize (func_equal m1 m2 fn bk br2 e s). rewrite func_equal.
+destruct (jump m2 fn bk br2 e s); simpl; eauto.
+apply jump_equal in func_equal. unfold jump_equal_trace_equiv in func_equal.
+specialize (func_equal m1 m2 fn bk br e s). rewrite func_equal.
+destruct (jump m2 fn bk br e s); simpl; eauto.
+Qed.
+
+
+
+
+Print fetch.
+
+
+
+Print find_block.
+Print block.
+
+Definition get_block (fid:function_id) (bid:block_id) (m:mcfg) : option block :=
+match find_function m fid with
+  | None => None
+  | Some fn => find_block (blks (df_instrs fn)) bid
+end.
+
+
+(*With the same fid, bid, m1 and m2 yield some result.
+The result, block_id are the same.
+block_phis are the same
+the stepD of the head of both are the same
+the tl of the code is the same
+the blk_term is also the same*)
+Print block.
+
+
+
+
+
+Definition block_same_phis (b1 b2:block) :=
+if (decide (b1.(blk_phis) = b2.(blk_phis))) then true else false.
+
+
+Definition block_same_id (b1 b2:block) :=
+if (decide (b1.(blk_id) = b2.(blk_id))) then true else false.
+
+
+
+Definition block_same_term (b1 b2: block) :=
+if (decide (b1.(blk_term) = b2.(blk_term))) then true else false.
+
+Print code.
+
+
+
+
+Definition tl (c:code) :=
+match c with
+  | [::] => [::]
+  | _ :: t => t
+end.
+
+
+
+
+Definition block_same_tl_code (b1 b2: block) := if decide (tl (b1.(blk_code)) = tl (b2.(blk_code))) then true else false.
+
+
+Print block.
+
+Print find_block_entry.
+Print block_entry.
+
+Print find_block_entry.
+Print block_entry.
+Print find_function.
+
+
+(*Either the first instruction of a block is the first of the list, if the list is empty then the terminator*)
+Definition hdb (b:block) :=
+match b.(blk_code) with
+  | [::] => None
+  | h :: _ => Some h
+end.
+
+Print sem.
+Definition hd_block_equal m1 m2 fnid bkid b1 b2 := 
+match hdb b1, hdb b2 with
+  | None, None => False
+  | Some (h1, t1), Some (h2, t2) => forall e s mem, step_trace_exec 0 (sem m1 ((mk_pc fnid bkid h1, e, s))) mem = step_trace_exec 0 (sem m2 ((mk_pc fnid bkid h2, e, s))) mem
+  | _, _ => False
+end.
+Print hdb.
+
+Definition hd_fst_block_equal b1 b2 := 
+match hdb b1, hdb b2 with
+  | None, None => False
+  | Some (h1, t1), Some (h2, t2) => h1 = h2
+  | _, _ => False
+end.
+
+
+
+
+Definition tl_block_equal b1 b2 :=
+tl (b1.(blk_code)) = tl (b2.(blk_code)).
+Print fst.
+Print hd.
+
+Definition list_equal (b:block) :=
+match hdb b with
+  | None => [::]
+  | Some h => (h :: tl b.(blk_code))
+end.
+
+
+Definition head (b:block) :=
+match b.(blk_code) with
+  | [::] => [::]
+  | h :: t => [::h]
+end.
+Print find_function.
+Print definition.
+Print cfg.
+
+(*(if (decide (fn1.(df_prototype) = fn2.(df_prototype))) then True else False) /\*)
+
+
+Definition fulldefinition (m1 m2: mcfg) :=
+forall fnid fn1 fn2, 
+(*Fetching a function_id (fnid) always returns some result*)
+(find_function m1 fnid = Some fn1) /\ (find_function m2 fnid = Some fn2) /\
+
+(*These bits of definition are all equal*)
+
+(*ADD DF_PROTOTYPE*)
+(if (decide (fn1.(df_args) = fn2.(df_args))) then True else False) /\
+
+
+(*Convert definition to CFG*)
+forall cfg cfg1, (df_instrs fn1) = cfg /\ (df_instrs fn2) = cfg1 /\
+(if (decide ((init cfg) = (init cfg1))) then True else False) /\
+(*These bits of the CFG are all equal*)
+
+forall bkid bk1 bk2,
+(*Fetching a block_id (bkid) always returns some result*)
+(find_block (blks (df_instrs fn1)) bkid = Some bk1) /\ (find_block (blks (df_instrs fn2)) bkid = Some bk2) /\
+
+
+(*The blk_id, blk_phis and the blk_term are all equal*)
+(if (decide (bk1.(blk_id) = bk2.(blk_id))) then True else False) /\
+(if (decide (bk1.(blk_phis) = bk2.(blk_phis))) then True else False) /\
+(if (decide (bk1.(blk_term) = bk2.(blk_term))) then True else False) /\
+hd_fst_block_equal bk1 bk2 /\
+
+
+(*The execution of the head of both blocks are equal*)
+hd_block_equal m1 m2 fnid bkid bk1 bk2 /\
+
+
+(*The body of both blocks are equal *)
+tl_block_equal bk1 bk2 /\
+
+bk1.(blk_code) = head bk1 ++ tl bk1.(blk_code) /\
+bk2.(blk_code) = head bk2 ++ tl bk2.(blk_code)
+
+.
+
+Lemma test123 : forall prog prog1, fulldefinition prog prog1 -> forall st mem, trace_equiv (memD mem (sem prog st)) (memD mem (sem prog1 st)).
+Proof. intros prog prog1 H. pcofix CIH.
+intros. pfold.
+
+
+assert ((memD mem (sem prog st)) = unroll (memD mem (sem prog st))).
+destruct (memD mem (sem prog st)); eauto. rewrite H0. clear H0.
+
+assert ((memD mem (sem prog1 st)) = unroll (memD mem (sem prog1 st))).
+destruct (memD mem (sem prog1 st)); eauto. rewrite H0. clear H0.
+
+
+destruct st. destruct p. destruct p.
+generalize H. intros. unfold fulldefinition in H0.
+specialize (H0 fn). simpl.
+
+remember (find_function prog fn) as find_func_fn.
+remember (find_function prog1 fn) as find_func_fn1.
+
+destruct find_func_fn, find_func_fn1; simpl in *; eauto.
++specialize (H0 d d0). destruct H0. clear H0. destruct H1. clear H0.
+unfold is_left in *. destruct (decide (df_args d = df_args d0)).
+destruct H1. 
+clear H0.
+remember (find_block (blks (df_instrs d)) bk) as find_block_fn.
+remember (find_block (blks (df_instrs d0)) bk) as find_block_fn1.
+destruct find_block_fn, find_block_fn1. unfold block_to_cmd.
+specialize (H1 (df_instrs d) (df_instrs d0)). destruct H1. clear H0. destruct H1. clear H0.
+destruct d. simpl in *. destruct (decide (init df_instrs = init (Ollvm_ast.df_instrs d0))).
+simpl in *. destruct H1. clear H0. specialize (H1 bk). unfold blk_term_id in *.
+unfold blk_term in *. simpl in *. specialize (H1 b b0). destruct H1. clear H0. destruct H1. clear H0.
+destruct b, b0. simpl in *.
+unfold hd_fst_block_equal in *. unfold tl_block_equal in *. simpl in *.
+destruct (decide (blk_id = blk_id0)), (decide (blk_phis = blk_phis0)), 
+(decide (blk_term = blk_term0)).
+
+destruct H1. clear H0. destruct H1. clear H0. destruct H1.
+clear H0.
+destruct H1. destruct H1. destruct H2.
+destruct H3. subst. unfold hd_block_equal in H1.
+unfold hdb in *. simpl in *. destruct blk_code, blk_code0; simpl in *; eauto; try inversion H1.
+destruct p. inversion H0. destruct p, p0. subst.
+destruct blk_term0. simpl in *. specialize (H1 e s mem).
+destruct (decide (i = pt)), (decide (pt = i1)); simpl in *; eauto.
+admit. admit. rewrite <- Heqfind_func_fn in H1. destruct df_instrs. simpl in *.
+rewrite <- Heqfind_block_fn in H1. unfold block_to_cmd in H1. unfold blk_term_id in H1.
+simpl in *.
+
+rewrite <- Heqfind_func_fn1 in H1. unfold block_to_cmd in H1. unfold blk_term_id in H1.
+rewrite <- Heqfind_block_fn1 in H1. unfold blk_term in H1. simpl in H1.
+destruct (decide (i = i1)), (decide (i1 = i1)); simpl in *; subst; simpl in *.
+admit. admit.
+
+
+
+
+
+remember (match i1 with
+           | IId id =>
+               match i2 with
+               | INSTR_Op op =>
+                   do dv <- eval_op e None op;
+                   Step
+                     ({| fn := fn; bk := bk; pt := fallthrough blk_code0 i |},
+                     add_env id dv e, s)
+               | INSTR_Call (_, ID_Global fid) args =>
+                   do fnentry <-
+                   trywith ("stepD: no function " ++ string_of fid)
+                     (find_function_entry prog1 fid);
+                   let
+                   'FunctionEntry ids pc_f := fnentry in
+                    do dvs <-
+                    map_monad (fun '(t, op) => eval_op e (Some t) op) args;
+                    Step
+                      (pc_f, combine ids dvs,
+                      KRet e id
+                        {| fn := fn; bk := bk; pt := fallthrough blk_code0 i |}
+                      :: s)
+               | INSTR_Call (_, ID_Local _) _ => t_raise "INSTR_Call to local"
+               | INSTR_Alloca t _ _ =>
+                   Obs
+                     (Eff
+                        (Alloca t
+                           (fun a : value =>
+                            ({|
+                             fn := fn;
+                             bk := bk;
+                             pt := fallthrough blk_code0 i |}, 
+                            add_env id a e, s))))
+               | INSTR_Load _ _ (u, ptr) _ =>
+                   do dv <- eval_op e (Some u) ptr;
+                   match dv with
+                   | DV _ => t_raise "ERROR: Load got non-pointer value"
+                   | DVALUE_CodePointer _ =>
+                       t_raise "ERROR: Load got non-pointer value"
+                   | DVALUE_Addr a =>
+                       Obs
+                         (Eff
+                            (Load a
+                               (fun dv0 : value =>
+                                ({|
+                                 fn := fn;
+                                 bk := bk;
+                                 pt := fallthrough blk_code0 i |},
+                                add_env id dv0 e, s))))
+                   | DVALUE_I1 _ => t_raise "ERROR: Load got non-pointer value"
+                   | DVALUE_I32 _ => t_raise "ERROR: Load got non-pointer value"
+                   | DVALUE_I64 _ => t_raise "ERROR: Load got non-pointer value"
+                   | DVALUE_Poison => t_raise "ERROR: Load got non-pointer value"
+                   end
+               | INSTR_Store _ _ _ _ => t_raise "ERROR: Store to non-void ID"
+               | INSTR_Fence => t_raise "Unsupported LLVM intsruction"
+               | INSTR_AtomicCmpXchg => t_raise "Unsupported LLVM intsruction"
+               | INSTR_AtomicRMW => t_raise "Unsupported LLVM intsruction"
+               | INSTR_Unreachable => t_raise "IMPOSSIBLE: unreachable"
+               | INSTR_VAArg => t_raise "Unsupported LLVM intsruction"
+               | INSTR_LandingPad => t_raise "Unsupported LLVM intsruction"
+               end
+           | IVoid _ =>
+               match i2 with
+               | INSTR_Op _ => t_raise "ID / Instr mismatch void/non-void"
+               | INSTR_Call (ret_ty, ID_Global fid) args =>
+                   do fnentry <-
+                   trywith ("stepD: no function " ++ string_of fid)
+                     (find_function_entry prog1 fid);
+                   let
+                   'FunctionEntry ids pc_f := fnentry in
+                    do dvs <-
+                    map_monad (fun '(t, op) => eval_op e (Some t) op) args;
+                    match ret_ty with
+                    | TYPE_I _ => t_raise "Call mismatch void/non-void"
+                    | TYPE_Pointer _ => t_raise "Call mismatch void/non-void"
+                    | TYPE_Void =>
+                        Step
+                          (pc_f, combine ids dvs,
+                          KRet_void e
+                            {| fn := fn; bk := bk; pt := fallthrough blk_code0 i |}
+                          :: s)
+                    | TYPE_Half => t_raise "Call mismatch void/non-void"
+                    | TYPE_Float => t_raise "Call mismatch void/non-void"
+                    | TYPE_Double => t_raise "Call mismatch void/non-void"
+                    | TYPE_X86_fp80 => t_raise "Call mismatch void/non-void"
+                    | TYPE_Fp128 => t_raise "Call mismatch void/non-void"
+                    | TYPE_Ppc_fp128 => t_raise "Call mismatch void/non-void"
+                    | TYPE_Metadata => t_raise "Call mismatch void/non-void"
+                    | TYPE_X86_mmx => t_raise "Call mismatch void/non-void"
+                    | TYPE_Array _ _ => t_raise "Call mismatch void/non-void"
+                    | TYPE_Function _ _ => t_raise "Call mismatch void/non-void"
+                    | TYPE_Struct _ => t_raise "Call mismatch void/non-void"
+                    | TYPE_Packed_struct _ => t_raise "Call mismatch void/non-void"
+                    | TYPE_Opaque => t_raise "Call mismatch void/non-void"
+                    | TYPE_Vector _ _ => t_raise "Call mismatch void/non-void"
+                    | TYPE_Identified _ => t_raise "Call mismatch void/non-void"
+                    end
+               | INSTR_Call (ret_ty, ID_Local _) _ => t_raise "INSTR_Call to local"
+               | INSTR_Alloca _ _ _ => t_raise "ID / Instr mismatch void/non-void"
+               | INSTR_Load _ _ _ _ => t_raise "ID / Instr mismatch void/non-void"
+               | INSTR_Store _ (t, val) (u, ptr) _ =>
+                   do dv <- eval_op e (Some t) val;
+                   do v <- eval_op e (Some u) ptr;
+                   match v with
+                   | DV _ => t_raise "ERROR: Store got non-pointer value"
+                   | DVALUE_CodePointer _ =>
+                       t_raise "ERROR: Store got non-pointer value"
+                   | DVALUE_Addr a =>
+                       Obs
+                         (Eff
+                            (Store a dv
+                               (fun _ : value =>
+                                ({|
+                                 fn := fn;
+                                 bk := bk;
+                                 pt := fallthrough blk_code0 i |}, e, s))))
+                   | DVALUE_I1 _ => t_raise "ERROR: Store got non-pointer value"
+                   | DVALUE_I32 _ => t_raise "ERROR: Store got non-pointer value"
+                   | DVALUE_I64 _ => t_raise "ERROR: Store got non-pointer value"
+                   | DVALUE_Poison => t_raise "ERROR: Store got non-pointer value"
+                   end
+               | INSTR_Fence => t_raise "Unsupported LLVM intsruction"
+               | INSTR_AtomicCmpXchg => t_raise "Unsupported LLVM intsruction"
+               | INSTR_AtomicRMW => t_raise "Unsupported LLVM intsruction"
+               | INSTR_Unreachable => t_raise "IMPOSSIBLE: unreachable"
+               | INSTR_VAArg => t_raise "Unsupported LLVM intsruction"
+               | INSTR_LandingPad => t_raise "Unsupported LLVM intsruction"
+               end
+           end) as TEST.
+
+
+remember (           match i1 with
+           | IId id =>
+               match i0 with
+               | INSTR_Op op =>
+                   do dv <- eval_op e None op;
+                   Step
+                     ({| fn := fn; bk := bk; pt := fallthrough blk_code0 i |},
+                     add_env id dv e, s)
+               | INSTR_Call (_, ID_Global fid) args =>
+                   do fnentry <-
+                   trywith ("stepD: no function " ++ string_of fid)
+                     (find_function_entry prog fid);
+                   let
+                   'FunctionEntry ids pc_f := fnentry in
+                    do dvs <-
+                    map_monad (fun '(t, op) => eval_op e (Some t) op) args;
+                    Step
+                      (pc_f, combine ids dvs,
+                      KRet e id
+                        {| fn := fn; bk := bk; pt := fallthrough blk_code0 i |}
+                      :: s)
+               | INSTR_Call (_, ID_Local _) _ => t_raise "INSTR_Call to local"
+               | INSTR_Alloca t _ _ =>
+                   Obs
+                     (Eff
+                        (Alloca t
+                           (fun a : value =>
+                            ({|
+                             fn := fn;
+                             bk := bk;
+                             pt := fallthrough blk_code0 i |}, 
+                            add_env id a e, s))))
+               | INSTR_Load _ _ (u, ptr) _ =>
+                   do dv <- eval_op e (Some u) ptr;
+                   match dv with
+                   | DV _ => t_raise "ERROR: Load got non-pointer value"
+                   | DVALUE_CodePointer _ =>
+                       t_raise "ERROR: Load got non-pointer value"
+                   | DVALUE_Addr a =>
+                       Obs
+                         (Eff
+                            (Load a
+                               (fun dv0 : value =>
+                                ({|
+                                 fn := fn;
+                                 bk := bk;
+                                 pt := fallthrough blk_code0 i |},
+                                add_env id dv0 e, s))))
+                   | DVALUE_I1 _ => t_raise "ERROR: Load got non-pointer value"
+                   | DVALUE_I32 _ => t_raise "ERROR: Load got non-pointer value"
+                   | DVALUE_I64 _ => t_raise "ERROR: Load got non-pointer value"
+                   | DVALUE_Poison => t_raise "ERROR: Load got non-pointer value"
+                   end
+               | INSTR_Store _ _ _ _ => t_raise "ERROR: Store to non-void ID"
+               | INSTR_Fence => t_raise "Unsupported LLVM intsruction"
+               | INSTR_AtomicCmpXchg => t_raise "Unsupported LLVM intsruction"
+               | INSTR_AtomicRMW => t_raise "Unsupported LLVM intsruction"
+               | INSTR_Unreachable => t_raise "IMPOSSIBLE: unreachable"
+               | INSTR_VAArg => t_raise "Unsupported LLVM intsruction"
+               | INSTR_LandingPad => t_raise "Unsupported LLVM intsruction"
+               end
+           | IVoid _ =>
+               match i0 with
+               | INSTR_Op _ => t_raise "ID / Instr mismatch void/non-void"
+               | INSTR_Call (ret_ty, ID_Global fid) args =>
+                   do fnentry <-
+                   trywith ("stepD: no function " ++ string_of fid)
+                     (find_function_entry prog fid);
+                   let
+                   'FunctionEntry ids pc_f := fnentry in
+                    do dvs <-
+                    map_monad (fun '(t, op) => eval_op e (Some t) op) args;
+                    match ret_ty with
+                    | TYPE_I _ => t_raise "Call mismatch void/non-void"
+                    | TYPE_Pointer _ => t_raise "Call mismatch void/non-void"
+                    | TYPE_Void =>
+                        Step
+                          (pc_f, combine ids dvs,
+                          KRet_void e
+                            {| fn := fn; bk := bk; pt := fallthrough blk_code0 i |}
+                          :: s)
+                    | TYPE_Half => t_raise "Call mismatch void/non-void"
+                    | TYPE_Float => t_raise "Call mismatch void/non-void"
+                    | TYPE_Double => t_raise "Call mismatch void/non-void"
+                    | TYPE_X86_fp80 => t_raise "Call mismatch void/non-void"
+                    | TYPE_Fp128 => t_raise "Call mismatch void/non-void"
+                    | TYPE_Ppc_fp128 => t_raise "Call mismatch void/non-void"
+                    | TYPE_Metadata => t_raise "Call mismatch void/non-void"
+                    | TYPE_X86_mmx => t_raise "Call mismatch void/non-void"
+                    | TYPE_Array _ _ => t_raise "Call mismatch void/non-void"
+                    | TYPE_Function _ _ => t_raise "Call mismatch void/non-void"
+                    | TYPE_Struct _ => t_raise "Call mismatch void/non-void"
+                    | TYPE_Packed_struct _ => t_raise "Call mismatch void/non-void"
+                    | TYPE_Opaque => t_raise "Call mismatch void/non-void"
+                    | TYPE_Vector _ _ => t_raise "Call mismatch void/non-void"
+                    | TYPE_Identified _ => t_raise "Call mismatch void/non-void"
+                    end
+               | INSTR_Call (ret_ty, ID_Local _) _ => t_raise "INSTR_Call to local"
+               | INSTR_Alloca _ _ _ => t_raise "ID / Instr mismatch void/non-void"
+               | INSTR_Load _ _ _ _ => t_raise "ID / Instr mismatch void/non-void"
+               | INSTR_Store _ (t, val) (u, ptr) _ =>
+                   do dv <- eval_op e (Some t) val;
+                   do v <- eval_op e (Some u) ptr;
+                   match v with
+                   | DV _ => t_raise "ERROR: Store got non-pointer value"
+                   | DVALUE_CodePointer _ =>
+                       t_raise "ERROR: Store got non-pointer value"
+                   | DVALUE_Addr a =>
+                       Obs
+                         (Eff
+                            (Store a dv
+                               (fun _ : value =>
+                                ({|
+                                 fn := fn;
+                                 bk := bk;
+                                 pt := fallthrough blk_code0 i |}, e, s))))
+                   | DVALUE_I1 _ => t_raise "ERROR: Store got non-pointer value"
+                   | DVALUE_I32 _ => t_raise "ERROR: Store got non-pointer value"
+                   | DVALUE_I64 _ => t_raise "ERROR: Store got non-pointer value"
+                   | DVALUE_Poison => t_raise "ERROR: Store got non-pointer value"
+                   end
+               | INSTR_Fence => t_raise "Unsupported LLVM intsruction"
+               | INSTR_AtomicCmpXchg => t_raise "Unsupported LLVM intsruction"
+               | INSTR_AtomicRMW => t_raise "Unsupported LLVM intsruction"
+               | INSTR_Unreachable => t_raise "IMPOSSIBLE: unreachable"
+               | INSTR_VAArg => t_raise "Unsupported LLVM intsruction"
+               | INSTR_LandingPad => t_raise "Unsupported LLVM intsruction"
+               end
+           end) as TEST1.
+
+
+
+
+
+
+
+
+
+
+
+
+
+
+
+
+
+
+
+destruct i0, i2. inversion H1.
+destruct (eval_op e None op), (eval_op e None op0); simpl in *; eauto.
+inversion H1. admit. constructor. left.
+assert ((memD mem
+     (trace_map (fun _ : state => ())
+        (step_sem prog1
+           ({| fn := fn; bk := bk; pt := fallthrough blk_code0 i |},
+           add_env id v0 e, s)))) = unroll (memD mem
+     (trace_map (fun _ : state => ())
+        (step_sem prog1
+           ({| fn := fn; bk := bk; pt := fallthrough blk_code0 i |},
+           add_env id v0 e, s))))).
+destruct (memD mem
+     (trace_map (fun _ : state => ())
+        (step_sem prog1
+           ({| fn := fn; bk := bk; pt := fallthrough blk_code0 i |},
+           add_env id v0 e, s)))); eauto. rewrite H0. clear H0.
+
+assert   ((memD mem
+     (trace_map (fun _ : state => ())
+        (step_sem prog
+           ({| fn := fn; bk := bk; pt := fallthrough blk_code0 i |},
+           add_env id v e, s)))) = unroll   (memD mem
+     (trace_map (fun _ : state => ())
+        (step_sem prog
+           ({| fn := fn; bk := bk; pt := fallthrough blk_code0 i |},
+           add_env id v e, s))))).
+destruct   (memD mem
+     (trace_map (fun _ : state => ())
+        (step_sem prog
+           ({| fn := fn; bk := bk; pt := fallthrough blk_code0 i |},
+           add_env id v e, s)))); eauto.
+rewrite H0. clear H0. simpl. rewrite <- Heqfind_func_fn. destruct df_instrs. simpl in *.
+
+induction i1, i0, i2; simpl in *; eauto. 
+destruct (eval_op e None op),(eval_op e None op0); simpl in *; eauto.
+simpl in *. eauto.
+rewrite <- Heqfind_func_fn1 in H1.
+
+destruct df_instrs. simpl in *. 
+rewrite <- Heqfind_block_fn1 in H1. unfold block_to_cmd in H1. unfold blk_term_id in *. unfold blk_term in H1. simpl in *. subst.
+destruct (decide (i = fallthrough blk_code0 i)), (decide (fallthrough blk_code0 i = IId id)). subst; simpl in *; eauto. rewrite <- e0 in e1. admit.
+simpl in *.
+
++specialize (H0 d d). destruct H0. destruct H1. inversion H1.
++specialize (H0 d d). destruct H0. inversion H0.
+Admitted.
