src/coq/optimisations/donothing.v
@@ -73,6 +73,9 @@ destruct p.
 simpl.
 unfold CFG.fetch.
 
+
+
+
 destr_simpl (CFG.find_function prog fn) CIH.
 destr_simpl d CIH. 
 destr_simpl df_instrs CIH.
