src/coq/optimisations/step_trace.v
@@ -1,0 +1,52 @@
+Require Import ZArith List String Omega.
+Require Import  Vellvm.Ollvm_ast Vellvm.Classes Vellvm.Util Vellvm.CFGProp Vellvm.CFG.
+Require Import Vellvm.optimisations.wellformedSSA.
+Require Import Vellvm.optimisations.transform.
+Require Import Vellvm.optimisations.add_instr.
+Require Import Vellvm.optimisations.paco_util.
+Require Import Vellvm.DecidableEquality.
+Require Import paco.
+Require Import Vellvm.Memory.
+Require Import Vellvm.Effects.
+From mathcomp.ssreflect
+Require Import ssreflect ssrbool seq eqtype ssrnat.
+
+Set Implicit Arguments.
+
+Print mcfg.
+Print Trace.
+Inductive finish_item X :=
+  | tauitem : X -> finish_item X
+  | visitem : Event (Trace X) -> finish_item X.
+
+Print Trace.
+
+Print Event.
+
+
+Fixpoint step_trace_exec (n:nat) (t:Trace ()) (m:memory) : option (finish_item ()) :=
+match n with
+  | 0 => match t with
+       | Vis (Eff e) =>
+                        match mem_step e m with
+                         | inr (m', v, k) => Some (tauitem tt)
+                         | inl _ => None
+                        end
+       | Vis a => Some (visitem (a))
+       | Tau a _ => Some (tauitem a)
+       end
+  | b.+1 => match t with
+       | Vis (Eff e) =>
+                        match mem_step e m with
+                         | inr (m', v, k) => step_trace_exec b (k v) m'
+                         | inl _ => None
+                        end
+       | Vis a => Some (visitem (a))
+       | Tau a d => step_trace_exec b d m
+       end
+end.
+
+
+(*COMPARE STEP_TRACE*)
+
+
